\documentclass{article}
\usepackage[utf8]{inputenc}
\usepackage{mathtools}

\title{Trajectory Estimator}
\author{Jake Timothy}
\date{April 2015}

\begin{document}

\maketitle

\section{Introduction}

\section{Batch Processor}
\subsection{Data}
\subsubsection{On-board Data}
\subsubsection{Off-board Data}

\subsection{State Estimator}

\section{Models}
\subsection{Gravity Model: World Geodetic System 1984}
\subsubsection{Spherical Harmonic Gravity Model}
\subsubsection{Spherical Harmonic Functions}
\subsubsection{Associated Legendre Polynomials}
\begin{equation}
T{\left(r,\theta,\lambda\right)} = \frac{G M}{r} \sum_{n=2}^\infty \left(\frac{a}{r}\right)^n \sum_{m=-n}^n \overline{C}_{n m}^s \overline{Y}_{n m}{\left(\theta,\lambda\right)}
\end{equation}

\begin{equation}
\overline{Y}_{n m}{\left(\theta,\lambda\right)} = \overline{P}_{n |m|}{\left(cos \theta\right)} \left\{\begin{array}{l}
cos m \lambda \\
sin |m| \lambda
\end{array}\right\} \begin{array}{l}
m \geq 0 \\
m < 0
\end{array}
\end{equation}

\begin{equation}
\overline{P}_{n m}{\left(x\right)} = \left(-1\right)^m \sqrt{\frac{\left(n + \frac{1}{2}\right) \left(n - m\right)!}{\left(n + m\right)!}} P_{n m}{\left(x\right)}
\end{equation}

\begin{equation}
P_{n m}{\left(x\right)} = \left\{\begin{array}{l}
\left(-1\right)^m \left(1 - x^2\right)^{m / 2} \frac{d^m}{d x^m} P_n{\left(x\right)} \\
\left(-1\right)^m \frac{\left(n - |m|\right)!}{\left(n + |m|\right)!} P_{n |m|}{\left(x\right)}
\end{array}\right\} \begin{array}{l}
m \geq 0 \\
m < 0
\end{array}
\end{equation}

\begin{equation}
P_n{\left(x\right)} = \frac{1}{2^n n!} \frac{d^n}{d x^n} \left(x^2 - 1\right)^n
\end{equation}

\begin{equation}
\overline{P}_{n m}{\left(x\right)} = \left\{\begin{array}{l}
\sqrt{\frac{\left(n + \frac{1}{2}\right) \left(n - m\right)!}{\left(n + m\right)!}} \left(1 - x^2\right)^{m / 2} \frac{d^m}{d x^m} P_n{\left(x\right)} \\
\left(-1\right)^m P_{n |m|}{\left(x\right)}
\end{array}\right\} \begin{array}{l}
m \geq 0 \\
m < 0
\end{array}
\end{equation}

\begin{equation}
P_{n m}{\left(x\right)} = \left(-1\right)^m \sqrt{\frac{\left(n + m\right)!}{\left(n + \frac{1}{2}\right) \left(n - m\right)!}} \overline{P}_{n m}{\left(x\right)}
\end{equation}

\begin{equation}
P_{n m}{\left(x\right)} = \left\{\begin{array}{l}
\left(-1\right)^m \sqrt{\frac{\left(n + m\right)!}{\left(n + \frac{1}{2}\right) \left(n - m\right)!}} \overline{P}_{n m}{\left(x\right)} \\
\sqrt{\frac{\left(n - |m|\right)!}{\left(n + \frac{1}{2}\right) \left(n + |m|\right)!}} \overline{P}_{n |m|}{\left(x\right)}
\end{array}\right\} \begin{array}{l}
m \geq 0 \\
m < 0
\end{array}
\end{equation}

\subsection{Atmosphere Model: U.S. Standard Atmosphere 1976}


\end{document}
